src/tls/Concrete.fst
@@ -1,0 +1,5 @@
+module IdealFlags
+let ideal_Nonce = false  
+let ideal_Sig = false 
+let ideal_PMS = false 
+let ideal_PRF = false 
