src/tls/Ideal.fst
@@ -1,0 +1,6 @@
+module IdealFlags
+
+assume val ideal_Nonce : bool  
+assume val ideal_Sig : bool 
+assume val ideal_PMS : bool 
+assume val ideal_PRF : bool 
